algebra/cmra.v
@@ -326,6 +326,8 @@ Lemma exclusive_l x `{!Exclusive x} y : ✓ (x ⋅ y) → False.
 Proof. by move /cmra_valid_validN /(_ 0) /exclusive0_l. Qed.
 Lemma exclusive_r x `{!Exclusive x} y : ✓ (y ⋅ x) → False.
 Proof. rewrite comm. by apply exclusive_l. Qed.
+Lemma exclusiveN_opM n x `{!Exclusive x} my : ✓{n} (x ⋅? my) → my = None.
+Proof. destruct my. move=> /(exclusiveN_l _ x) []. done. Qed.
 
 (** ** Order *)
 Lemma cmra_included_includedN n x y : x ≼ y → x ≼{n} y.
@@ -965,6 +967,8 @@ Section option.
   Definition Some_op a b : Some (a ⋅ b) = Some a ⋅ Some b := eq_refl.
   Lemma Some_core `{CMRATotal A} a : Some (core a) = core (Some a).
   Proof. rewrite /core /=. by destruct (cmra_total a) as [? ->]. Qed.
+  Lemma Some_op_opM x my : Some x ⋅ my = Some (x ⋅? my).
+  Proof. by destruct my. Qed.
 
   Lemma option_included (mx my : option A) :
     mx ≼ my ↔ mx = None ∨ ∃ x y, mx = Some x ∧ my = Some y ∧ (x ≼ y ∨ x ≡ y).
